



$$1a) \quad x^2 - 9 > 0 \Leftrightarrow x^2 > 9 \Leftrightarrow x > 3 \\ x < -3$$

$$D_f = ]-\infty, -3[ \cup ]3, +\infty[$$

$$b) \quad 2x - 3 \neq 0 \Leftrightarrow 2x \neq 3 \Leftrightarrow x \neq \frac{3}{2}$$

$$x + 1 \geq 0 \Leftrightarrow x \geq -1$$

$$D_g = [-1, \frac{3}{2}[ \cup ]\frac{3}{2}, +\infty[$$

$$2a) \quad \frac{x^2 - 9}{x^2 - 5x + 6} = \frac{(\cancel{x-3})(x+3)}{(\cancel{x-3})(x-2)} = \frac{x+3}{x-2} = \frac{3+3}{3-2} = 6$$

$$b) \quad \frac{3x^3 - 2x + 1}{6x^3 + x^2 - 4} = \frac{3 - \frac{2}{x^2} + \frac{1}{x^3}}{6 + \frac{1}{x} - \frac{4}{x^4}} = \frac{3}{6} = \frac{1}{2}$$

$$c) \quad \frac{\sqrt{1+x} - 1}{x} =$$

$$3) \quad f(x) = \frac{x^2 - 4}{x - 2} = \frac{(\cancel{x-2})(x+2)}{\cancel{x-2}} = x + 2 = 2 + 2 = 4$$

$$K = 4$$

4)

$$h(0) = x^3 - 3x + 1 = 0^3 - 3(0) + 1 = 1$$

$$h(1) = x^3 - 3x + 1 = 1^3 - 3(1) + 1 = -1$$

$$h(0) = 1 > 0$$

$$h(1) = -1 < 0$$

$$5) \quad x + 2 > 0 \Leftrightarrow x > -2 \quad D_f: ]-\infty, -2[ \cup ]-2, +\infty[$$

$$f(2^+) = \frac{2x^2 + x - 1}{x + 2} = \frac{2(2^+)^2 + 2^+ - 1}{2 + 2} = \frac{8 + 2 - 1}{0^+} = \frac{9}{0^+} = +\infty$$

$$f(2^-) = \frac{2x^2 + x - 1}{x + 2} = \frac{2(2^-)^2 + 2^- - 1}{2 + 2} = \frac{8 + 2 - 1}{0^-} = \frac{9}{0^-} = -\infty$$

$$m = \lim_{x \rightarrow +\infty} \frac{2x^2 + x - 1}{x^2 + 2} = \frac{2 + \frac{1}{x} - \frac{1}{x^2}}{\frac{1}{x} + \frac{2}{x^2}} = \frac{2 + 0 - 0}{0} = 2$$

$$b = \lim_{x \rightarrow +\infty} \frac{2x^2 + x - 1}{x + 2} - 2x = \frac{2x^2 + x - 1 - 2x(x + 2)}{x + 2} = \frac{2x^2 + x - 1 - 2x^2 - 4x}{x + 2}$$

$$= \frac{5x - 1}{x + 2} = \frac{5 - \frac{1}{x}}{\frac{1}{x} + \frac{2}{x}} = \frac{5 - 0}{0 + 0} = 5$$

$$y = 2x - (2 - 2(2)) = 2x - (2 - 4) = 2x + 2$$

$$AV = 2$$

$$AH = \text{New term } \frac{\text{gram } 2^-}{\text{gram } 1^2}$$

$$AO = 2x + 2$$

$$6a) f'(x) = \frac{3x(x^2 - 2) - 2x(3x + 1)}{(x^2 - 2)^2} = \frac{3x^3 - 6 - 5x + 2}{x^4 - 4}$$

$$b) g'(x) = \ln(x^3 + 2x - 1)$$

$$c) h'(x) = -\sin(x) \cdot e^{2x} + \cos(x) \times 2e^{2x}$$

$$7a) \int 4x^3 - 6x + 5 \, dx = \frac{4x^4}{4} - \frac{6x^2}{2} + 5x + C, C \in \mathbb{R}$$

$$b) \int \frac{6x^2}{x^3+4} \, dx = 2 \ln(x^3+4) + C, C \in \mathbb{R}$$

$$c) \int x \cdot \cos(x) \, dx = x \cdot \sin(x) - \int \sin(x) \, dx = x \cdot \sin(x) - \cos(x) + C, C \in \mathbb{R}$$

$$8) \int x^2 + 2x - 1 \, dx = \left[ \frac{x^3}{3} + \frac{2x^2}{2} - x \right]_{-1}^2 =$$

$$\frac{2^3}{3} + \frac{2(2)^2}{2} - 2 - \left( \frac{(-1)^3}{3} + \frac{2(-1)^2}{2} - 1 \right) = \frac{8}{3} - \frac{8}{2} - \frac{2}{1} - \frac{-1}{3} + \frac{1}{2} + \frac{1}{1}$$

$$\frac{16}{6} - \frac{24}{6} - \frac{12}{6} - \frac{-2}{6} + \frac{3}{6} + \frac{6}{6} = \frac{-9}{6} = \frac{-3}{2}$$

9)

$$F(1) = \frac{6x^3}{3} - \frac{4x^2}{2} + C = 2x^3 - 2x^2 + C = 3, C=3$$

$$10) \quad x^2 = 3^2 = 9$$

$$2x + 3 = 9$$

$$A = \int_{-1}^3 x^2 - (2x + 3) \, dx = \left[ \frac{x^3}{3} - \left( \frac{2x^2}{2} + 3x \right) \right]_{-1}^3 =$$

$$A = \frac{3^3}{3} - \left( \frac{2(3)^2}{2} + 3(3) \right) - \frac{-1^3}{3} - \left( \frac{2(-1)^2}{2} + 3(-1) \right) =$$

$$A = \frac{27}{3} - \left( \frac{18}{2} + \frac{9}{1} \right) - \frac{-1}{3} - \left( \frac{2}{2} - \frac{3}{1} \right) =$$

$$A = \frac{27}{3} - \left( \frac{18}{2} + \frac{18}{2} \right) - \frac{-1}{3} - \left( \frac{2}{2} - \frac{6}{2} \right) =$$

$$A = \frac{27}{3} - \frac{36}{2} - \frac{-1}{3} + \frac{4}{2} =$$

$(\times 2) \quad (\times 3) \quad (\times 2) \quad (\times 3)$

$$A = \frac{54}{6} - \frac{108}{6} - \frac{-2}{6} + \frac{12}{6} = -\frac{40}{6}$$

$$A = -\frac{40}{6}$$